theories/Zm.v
@@ -28,6 +28,45 @@ Proof.
   simpl in H. destruct H. f_equal. apply proof_irrelevance.
 Qed.
 
+Lemma Zm_in_bounds_mod :
+  ∀ μ n,
+  μ ≠ 0 →
+  Zm_in_bounds μ (n mod Z.of_nat μ)%Z.
+Proof.
+  intros μ n H_μ. apply Z_mod_lt; lia.
+Qed.
+
+Lemma Zm_in_bounds_impl_mod :
+  ∀ μ n,
+  Zm_in_bounds μ n →
+  (n mod Z.of_nat μ)%Z = n.
+Proof.
+  intros μ n H. apply Zmod_small. auto.
+Qed.
+
+Lemma Zm_in_bounds_Zm {μ} :
+  μ ≠ 0 →
+  ∀ n : Zm μ, Zm_in_bounds μ (Zm_n n).
+Proof.
+  intros H_μ. destruct n as [n canonical_n]. simpl. unfold Zm_canonical in canonical_n.
+  specialize (canonical_n (- (n / Z.of_nat μ))%Z). rewrite Z.mul_opp_l, Z.add_opp_r, <- Zmod_eq_full in canonical_n by lia.
+  specialize (canonical_n (Zm_in_bounds_mod _ _ H_μ)). rewrite Z.eq_opp_l, Z.opp_0 in canonical_n.
+  apply Z.div_small_iff in canonical_n as [canonical_n | canonical_n].
+  - auto.
+  - lia.
+  - lia.
+Qed.
+
+Lemma eq_Zm {μ} :
+  ∀ n m : Zm μ, n = m ↔ (Zm_n n mod Z.of_nat μ)%Z = (Zm_n m mod Z.of_nat μ)%Z.
+Proof.
+  intros n m. split.
+  - intros <-. auto.
+  - intros H. apply irrelevant_Zm. destruct (classic (μ = 0)) as [-> | H_μ].
+    + rewrite ! Zmod_0_r in H. auto.
+    + rewrite ! (Zm_in_bounds_impl_mod _ _ (Zm_in_bounds_Zm H_μ _)) in H. auto.
+Qed.
+
 Lemma Zm_eq_dec {μ} :
   ∀ n m : Zm μ, {n = m} + {n ≠ m}.
 Proof.
@@ -37,14 +76,6 @@ Proof.
 Qed.
 
 Instance dec_eq_Zm {μ} : EqDec (Zm μ) eq := Zm_eq_dec.
-
-Lemma Zm_in_bounds_impl_mod :
-  ∀ μ n,
-  Zm_in_bounds μ n →
-  (n mod Z.of_nat μ)%Z = n.
-Proof.
-  intros μ n H. apply Zmod_small. auto.
-Qed.
 
 #[program]
 Definition Zm_of_Z {μ} (n : Z) : Zm μ := {|
@@ -66,4 +97,95 @@ Proof.
   intros n. apply irrelevant_Zm. simpl. rewrite Zmod_mod. auto.
 Qed.
 
+Lemma eq_Zm_of_Z {μ} :
+  ∀ n m, @Zm_of_Z μ n = @Zm_of_Z μ m ↔ (n mod Z.of_nat μ)%Z = (m mod Z.of_nat μ)%Z.
+Proof.
+  intros n m. split.
+  - ltac1:(intros [=H]). auto.
+  - intros H. apply irrelevant_Zm. auto.
+Qed.
+
 Compute Zm_of_Z 7 : Zm 3.
+
+Definition Zm_le {μ} (n m : Zm μ) := (Zm_n n ≤ Zm_n m)%Z.
+
+Lemma refl_Zm_le {μ} :
+  ∀ n : Zm μ, Zm_le n n.
+Proof.
+  intros n. unfold Zm_le. reflexivity.
+Qed.
+
+Lemma trans_Zm_le {μ} :
+  ∀ n m k : Zm μ, Zm_le n m → Zm_le m k → Zm_le n k.
+Proof.
+  intros n m k H_1 H_2. unfold Zm_le in *. apply transitivity with (Zm_n m); auto.
+Qed.
+
+Instance preorder_Zm_le {μ} : PreOrder (@Zm_le μ) :=
+  {| PreOrder_Reflexive := refl_Zm_le; PreOrder_Transitive := trans_Zm_le |}.
+
+Instance partial_order_Zm_le {μ} : PartialOrder eq (@Zm_le μ).
+Proof.
+  intros n m. unfold relation_conjunction, predicate_intersection, flip; simpl. split.
+  - intros <-. split; reflexivity.
+  - intros (H_1 & H_2). apply irrelevant_Zm. unfold Zm_le in H_1, H_2. lia.
+Qed.
+
+Instance total_Zm_le {μ} : Total (@Zm_le μ).
+Proof.
+  intros n m. unfold Zm_le. apply totality.
+Qed.
+
+Instance dec_le_Zm {μ} : DecLe (@Zm_le μ).
+Proof.
+  intros n m. unfold le, Zm_le. apply dec_le_Z.
+Defined.
+
+#[program]
+Definition infinite_Zm : infinite (Zm 0) :=
+  λ l, exist _ (Zm_of_Z (` (infinite_Z (List.map Zm_n l)))) _.
+Next Obligation.
+  intros l. remember (List.map Zm_n l) as l' eqn:H_l'. destruct (infinite_Z l') as (n & H_n); simpl.
+  subst l'. induction l as [| m l' IH].
+  - auto.
+  - intros [-> | H_l'].
+    + apply H_n. left. simpl. apply Zmod_0_r.
+    + apply IH.
+      * intros H. apply H_n. right. auto.
+      * auto.
+Qed.
+
+Fixpoint Zm_all_aux {μ} n : list (Zm μ) :=
+  match n with
+  | 0 => []
+  | S n' => Zm_of_Z (Z.of_nat n') :: Zm_all_aux n'
+  end.
+
+Definition Zm_all {μ} : list (Zm μ) := Zm_all_aux μ.
+
+Lemma list_In_Zm_all {μ} :
+  μ ≠ 0 →
+  ∀ n : Zm μ, List.In n Zm_all.
+Proof.
+  intros H_μ n. unfold Zm_all. specialize (Zm_in_bounds_Zm H_μ n) as H_n. assert (H_m : μ ≤ μ) by lia. induction μ as [| m IH] in H_n at 1, H_m at 1 |- * at 3.
+  - unfold Zm_in_bounds in H_n. lia.
+  - simpl. destruct (classic (Zm_of_Z (Z.of_nat m) = n)) as [<- | H].
+    + left. auto.
+    + right. unfold Zm_in_bounds in H_n, IH. apply IH.
+      * rewrite eq_Zm in H. simpl in H. rewrite Zmod_mod, Zmod_small in H by lia.
+        rewrite (Zm_in_bounds_impl_mod _ _ (Zm_in_bounds_Zm H_μ _)) in H. lia.
+      * lia.
+Qed.
+
+#[program]
+Definition finite_Zm {μ} (H_μ : μ ≠ 0) : finite (Zm μ) :=
+  exist _ Zm_all _.
+Next Obligation.
+  intros μ H_μ. simpl. apply list_In_Zm_all; auto.
+Qed.
+
+Instance dec_finite_Zm {μ} : DecFinite (Zm μ) :=
+  match μ == 0 with
+  | left H_μ => inr (rew <- [λ μ, infinite (Zm μ)] H_μ in infinite_Zm)
+  | right H_μ => inl (finite_Zm H_μ)
+  end.
